theories/iris/language/iris_resources.v
@@ -217,6 +217,8 @@ Notation "n ↦[we] v" := (pointsto (L:=N) (V:=exception) n (DfracOwn 1) v%V)
                              (at level 20, format "n ↦[we] v") : bi_scope.
 
 
+Notation "n ↦□[tag] v" := (pointsto (L:=N) (V:=function_type) n (DfracDiscarded) v%V)%I
+                           (at level 20, format "n ↦□[tag] v") : bi_scope.
 Notation "n ↦[tag]{ q } v" := (pointsto (L:=N) (V:=function_type) n q v%V)%I
                            (at level 20, format "n ↦[tag]{ q } v") : bi_scope.
 Notation "n ↦[tag] v" := (pointsto (L:=N) (V:=function_type) n (DfracOwn 1) v%V)%I
